test: add support for v1 and v2 manifests

TestVectors/dafny/TestVectors/src/ParseEsdkJsonManifest.dfy
@@ -37,6 +37,50 @@ module {:options "-functionSyntax:4"} ParseEsdkJsonManifest {
   const encryptionContextJsonKey := "encryption-context"
   const reproducedEncryptionContextJsonKey := "reproduced-encryption-context"
 
+  function BuildV1DecryptTestVector(
+    op: EsdkManifestOptions.ManifestOptions,
+    version: SupportedDecryptVersion,
+    keys: KeyVectors.KeyVectorsClient,
+    obj: seq<(string, JSON)>
+  ) : Result<seq<EsdkDecryptTestVector>, string>
+    requires op.V1Decrypt?
+  {
+    if |obj| == 0 then
+      Success([])
+    else
+      var tail :- BuildV1DecryptTestVector(op, version, keys, obj[1..]);
+      var decryptVector :- ToDecryptTestVectors(op, version, keys, obj[0].0, obj[0].1);
+      Success([ decryptVector ] + tail)
+  } by method {
+    // This function ideally would be`{:tailrecursion}`
+    // but it is not simple to here is a method
+    // so that it does not explode with huge numbers of tests.
+    var i: nat := |obj|;
+    var vectors := [];
+
+    while i != 0
+      decreases i
+      invariant Success(vectors) == BuildV1DecryptTestVector(op, version, keys, obj[i..])
+    {
+      i := i - 1;
+      var test := ToDecryptTestVectors(op, version, keys, obj[i].0, obj[i].1);
+      if test.Failure? {
+        ghost var j := i;
+        while j != 0
+          decreases j
+          invariant Failure(test.error) == BuildV1DecryptTestVector(op, version, keys, obj[j..])
+        {
+          j := j - 1;
+        }
+        return Failure(test.error);
+      }
+
+      vectors := [test.value] + vectors;
+    }
+
+    return Success(vectors);
+  }
+
   function BuildDecryptTestVector(
     op: EsdkManifestOptions.ManifestOptions,
     version: SupportedDecryptVersion,
@@ -82,20 +126,25 @@ module {:options "-functionSyntax:4"} ParseEsdkJsonManifest {
   }
 
 
-  function ToDecryptTestVectors(
+  function {:vcs_split_on_every_assert} ToDecryptTestVectors(
     op: EsdkManifestOptions.ManifestOptions,
     version: SupportedDecryptVersion,
     keys: KeyVectors.KeyVectorsClient,
     name: string,
     json: JSON
   ) : Result<EsdkDecryptTestVector, string>
-    requires op.Decrypt?
+    requires op.Decrypt? || op.V1Decrypt?
   {
     :- Need(json.Object?, "Vector is not an object");
     var obj := json.obj;
 
     match version
-    case 3 => V3ToDecryptTestVector(op, keys, name, obj, version)
+    case 3 =>
+      :- Need(op.Decrypt?, "Err parsing manifest expected Decrypt");
+      V3ToDecryptTestVector(op, keys, name, obj, version)
+    case 1 =>
+      :- Need(op.V1Decrypt?, "Err parsing manifest expected V1Decrypt");
+      V1ToDecryptTestVector(op, keys, name, obj, version)
     case _ => Failure("Version not supported")
 
     // case 1 =>
@@ -283,6 +332,40 @@ module {:options "-functionSyntax:4"} ParseEsdkJsonManifest {
 
   }
 
+  function V1ToDecryptTestVector(
+    op: EsdkManifestOptions.ManifestOptions,
+    keys: KeyVectors.KeyVectorsClient,
+    name: string,
+    obj: seq<(string, JSON)>,
+    version: SupportedDecryptVersion
+  ) : Result<EsdkDecryptTestVector, string>
+    requires op.V1Decrypt?
+  {
+    var plaintextLoc :- GetString("plaintext", obj);
+    var ciphertextLoc :- GetString("ciphertext", obj);
+    :- Need(
+         && "file://" < ciphertextLoc
+         && "file://" < plaintextLoc,
+         "Invalid file prefix in test vector"
+       );
+    var masterKeys :- GetArray("master-keys", obj);
+    var keyDescriptions :- GetKeyDescriptions(masterKeys, keys);
+    var keyDescription :- ToMultiKeyDescription(keyDescriptions);
+
+    Success(PositiveV1DecryptTestVector(
+              id := name,
+              version := version,
+              manifestPath := op.manifestPath,
+              ciphertextPath := ciphertextLoc[|FILE_PREPEND|..],
+              plaintextPath := plaintextLoc[|FILE_PREPEND|..],
+              decryptDescriptions := keyDescription,
+              frameLength := None,
+              algorithmSuiteId := None,
+              description :=  name,
+              decryptionMethod := DecryptionMethod.OneShot
+            ))
+  }
+
   function V3ToDecryptTestVector(
     op: EsdkManifestOptions.ManifestOptions,
     keys: KeyVectors.KeyVectorsClient,
@@ -348,6 +431,21 @@ module {:options "-functionSyntax:4"} ParseEsdkJsonManifest {
                                           .MapFailure(ParseJsonManifests.ErrorToString);
       var tail :- GetKeyDescriptions(keyArray[1..], keys);
       Success([encryptDecryptKeyDescription.keyDescription] + tail)
+  }
+
+  function ToMultiKeyDescription(keyDescriptions: seq<KeyVectorsTypes.KeyDescription>)
+    : Result<KeyVectorsTypes.KeyDescription, string>
+  {
+    if |keyDescriptions| == 1 then
+      Success(keyDescriptions[0])
+    else
+      :- Need(|keyDescriptions| > 1, "Received invalid key description length");
+      Success(KeyVectorsTypes.KeyDescription.Multi(
+                KeyVectorsTypes.MultiKeyring(
+                  generator := Some(keyDescriptions[0]),
+                  childKeyrings := keyDescriptions[1..]
+                )
+              ))
   }
 
   function GetPath(key: string, obj: seq<(string, JSON)>)
